refactor

BasicTyping.v
@@ -1,70 +1,50 @@
 From stdpp Require Import mapset.
-From CT Require Import CoreLangProp.
+From CT Require Import Syntax.Lang.
+From CT Require Import BaseDef.
+From CT Require Import Syntax.Primitives.
 
-Import Atom.
-Import CoreLang.
-Import Tactics.
-Import NamelessTactics.
-
-(** This file defines the basic type system of λᴱ. *)
-
-Definition ty_of_const (c: constant): base_ty :=
-  match c with
-  | cnat _ => TNat
-  | cbool _ => TBool
-  end.
-
-Definition ret_ty_of_op (op: effop): base_ty :=
-  match op with
-  | op_plus_one => TNat
-  | op_eq_zero => TBool
-  | op_rannat => TNat
-  end.
-
-Definition ty_of_op (op: effop): ty := TNat ⤍ (ret_ty_of_op op).
+Import BaseDef.
+Import Lang.
+Import Primitives.
 
 Definition context := amap ty.
 #[global]
 Instance context_stale : Stale context := dom.
 Arguments context_stale /.
 
-Reserved Notation "Γ '⊢t' t '⋮t' T" (at level 40).
-Reserved Notation "Γ '⊢t' t '⋮v' T" (at level 40).
-
 (** Basic typing rules  *)
 Inductive tm_has_type : context -> tm -> ty -> Prop :=
-| BtErr: forall Γ T, Γ ⊢t (terr T) ⋮t T
-| BtValue : forall Γ v T, Γ ⊢t v ⋮v T -> Γ ⊢t v ⋮t T
+| BtErr: forall Γ T, tm_has_type Γ (terr T) T
+| BtValue : forall Γ v T, value_has_type Γ v T -> tm_has_type Γ (treturn v) T
 | BtLetE : forall Γ e1 e2 T1 T2 (L: aset),
-    Γ ⊢t e1 ⋮t T1 ->
-    (forall (x: atom), x ∉ L -> (<[ x := T1]> Γ) ⊢t e2 ^t^ x ⋮t T2) ->
-    Γ ⊢t (tlete e1 e2) ⋮t T2
+    tm_has_type Γ e1 T1 ->
+    (forall (x: atom), x ∉ L -> tm_has_type (<[ x := T1]> Γ) (e2 ^^ x) T2) ->
+    tm_has_type Γ (tlete e1 e2) T2
 | BtEffOp : forall Γ (op: effop) v1 e (T1 Tx: base_ty) T (L: aset),
-    Γ ⊢t v1 ⋮v T1 ->
+    value_has_type Γ v1 T1 ->
     (ty_of_op op) = T1 ⤍ Tx ->
-    (forall (x: atom), x ∉ L -> (<[x := TBase Tx]> Γ) ⊢t e ^t^ x ⋮t T) ->
-    Γ ⊢t tleteffop op v1 e ⋮t T
+    (forall (x: atom), x ∉ L -> tm_has_type (<[x := TBase Tx]> Γ) (e ^^ x) T) ->
+    tm_has_type Γ (tleteffop op v1 e) T
 | BtApp : forall Γ v1 v2 e T1 Tx T (L: aset),
-    Γ ⊢t v1 ⋮v T1 ⤍ Tx ->
-    Γ ⊢t v2 ⋮v T1 ->
-    (forall (x: atom), x ∉ L -> (<[x := Tx]> Γ) ⊢t e ^t^ x ⋮t T) ->
-    Γ ⊢t tletapp v1 v2 e ⋮t T
+    value_has_type Γ v1 (T1 ⤍ Tx) ->
+    value_has_type Γ v2 T1 ->
+    (forall (x: atom), x ∉ L -> tm_has_type (<[x := Tx]> Γ) (e ^^ x) T) ->
+    tm_has_type Γ (tletapp v1 v2 e) T
 | BtMatchb: forall Γ v e1 e2 T,
-    Γ ⊢t v ⋮v TBool ->
-    Γ ⊢t e1 ⋮t T ->
-    Γ ⊢t e2 ⋮t T ->
-    Γ ⊢t (tmatchb v e1 e2) ⋮t T
+    value_has_type Γ v TBool ->
+    tm_has_type Γ e1 T ->
+    tm_has_type Γ e2 T ->
+    tm_has_type Γ (tmatchb v e1 e2) T
 with value_has_type : context -> value -> ty -> Prop :=
-| BtConst : forall Γ (c: constant), Γ ⊢t c ⋮v (ty_of_const c)
+| BtConst : forall Γ (c: constant), value_has_type Γ (vconst c) (ty_of_const c)
 | BtVar : forall Γ (x: atom) T,
-    Γ !! x = Some T -> Γ ⊢t x ⋮v T
+    Γ !! x = Some T -> value_has_type Γ (vfvar x) T
 | BtFun : forall Γ Tx T e (L: aset),
-    (forall (x: atom), x ∉ L -> (<[x := Tx]> Γ) ⊢t e ^t^ x ⋮t T) ->
-    Γ ⊢t vlam Tx e ⋮v Tx ⤍ T
+    (forall (x: atom), x ∉ L -> tm_has_type (<[x := Tx]> Γ) (e ^^ x) T) ->
+    value_has_type Γ (vlam Tx e) (Tx ⤍ T)
 | BtFix : forall Γ (Tx: base_ty) T e (L: aset),
-    (forall (x: atom), x ∉ L -> (<[x := TBase Tx]>Γ) ⊢t (vlam (Tx ⤍ T) e) ^v^ x ⋮v ((Tx ⤍ T) ⤍ T)) ->
-    Γ ⊢t vfix (Tx ⤍ T) (vlam (Tx ⤍ T) e) ⋮v Tx ⤍ T
-where "Γ '⊢t' t '⋮t' T" := (tm_has_type Γ t T) and "Γ '⊢t' t '⋮v' T" := (value_has_type Γ t T).
+    (forall (x: atom), x ∉ L -> tm_has_type (<[x := TBase Tx]>Γ) (vlam (Tx ⤍ T) e ^^ x) ((Tx ⤍ T) ⤍ T)) ->
+    value_has_type Γ (vfix (Tx ⤍ T) (vlam (Tx ⤍ T) e)) (Tx ⤍ T).
 
 Scheme value_has_type_mutual_rec := Induction for value_has_type Sort Prop
     with tm_has_type_mutual_rec := Induction for tm_has_type Sort Prop.
@@ -72,65 +52,10 @@ Scheme value_has_type_mutual_rec := Induction for value_has_type Sort Prop
 Global Hint Constructors tm_has_type: core.
 Global Hint Constructors value_has_type: core.
 
-(** * Naming related properties of the basic type system *)
+#[global]
+Instance has_normal_type_tm_instance : Typing context tm ty := tm_has_type.
+Arguments has_normal_type_tm_instance /.
 
-Lemma basic_typing_contains_fv_tm: forall Γ e T, Γ ⊢t e ⋮t T -> fv_tm e ⊆ dom Γ
-with basic_typing_contains_fv_value: forall Γ e T, Γ ⊢t e ⋮v T -> fv_value e ⊆ dom Γ.
-Proof.
-  all:
-  destruct 1; simpl; eauto;
-  try select (forall x, _ ∉ _ -> _) (fun H => auto_pose_fv x; repeat specialize_with x);
-  repeat select (_ ⊢t _ ⋮v _) (fun H => apply basic_typing_contains_fv_value in H);
-  repeat select (_ ⊢t _ ⋮t _) (fun H => apply basic_typing_contains_fv_tm in H);
-  simpl in *;
-  repeat
-    match goal with
-    | H : fv_tm ({_ ~t> _} _) ⊆ _ |- _ =>
-        setoid_rewrite <- open_fv_tm' in H
-    | H : _ ⊆ dom (<[_:=_]>_) |- _ =>
-        setoid_rewrite dom_insert in H
-    | H : _ !! _ = _ |- _ =>
-        apply elem_of_dom_2 in H
-    end;
-  my_set_solver.
-Qed.
-
-Lemma basic_typing_closed_tm: forall e T, ∅ ⊢t e ⋮t T -> closed_tm e.
-Proof.
-  intros.
-  apply basic_typing_contains_fv_tm in H. my_set_solver.
-Qed.
-
-Lemma basic_typing_closed_value: forall v T, ∅ ⊢t v ⋮v T -> closed_value v.
-Proof.
-  intros.
-  apply basic_typing_contains_fv_value in H. my_set_solver.
-Qed.
-
-Lemma basic_typing_regular_value: forall Γ v t, Γ ⊢t v ⋮v t -> lc v
-with basic_typing_regular_tm: forall Γ e t, Γ ⊢t e ⋮t t -> lc e.
-Proof.
-  all: destruct 1; simpl;
-    try econstructor; try instantiate_atom_listctx; eauto.
-Qed.
-
-Ltac lc_basic_typing_simp_aux :=
-  match goal with
-  | [H: _ ⊢t ?e ⋮t _ |- lc ?e] => apply basic_typing_regular_tm in H
-  | [H: _ ⊢t ?v ⋮v _ |- lc (treturn ?v)] => apply basic_typing_regular_value in H
-  | [H: _ ⊢t _ ⋮v _ |- lc _] => apply basic_typing_regular_value in H; simp_hyps
-  | [H: _ ⊢t _ ⋮t _ |- lc _] => apply basic_typing_regular_tm in H; simp_hyps
-  | [H: _ ⊢t _ ⋮v _ |- body _] => apply basic_typing_regular_value in H; simp_hyps
-  | [H: _ ⊢t _ ⋮t _ |- body _] => apply basic_typing_regular_tm in H; simp_hyps
-  | [H: _ ⊢t _ ⋮v _ |- context [fv_value _]] =>
-      apply basic_typing_closed_value in H; simp_hyps
-  | [H: _ ⊢t _ ⋮t _ |- context [fv_value _]] =>
-      apply basic_typing_closed_tm in H; simp_hyps
-  | [H: _ ⊢t _ ⋮v _ |- context [fv_tm _]] =>
-      apply basic_typing_closed_value in H; simp_hyps
-  | [H: _ ⊢t _ ⋮t _ |- context [fv_tm _]] =>
-      apply basic_typing_closed_tm in H; simp_hyps
-  end; eauto.
-
-Ltac basic_typing_regular_simp :=
-  repeat lc_basic_typing_simp_aux; eauto.
+#[global]
+Instance has_normal_type_value_instance : Typing context value ty := value_has_type.
+Arguments has_normal_type_value_instance /.
