BaseDef.v
@@ -1,0 +1,56 @@
+From stdpp Require Import stringmap mapset.
+From Stdlib Require Import Strings.String.
+
+(** This file defines atom, i.e., variable names, and its related concepts. *)
+
+(** We use strings as variables in the core langauge. *)
+Definition atom := string.
+Definition amap := stringmap.
+Definition aset := stringset.
+
+Definition atom_dec: ∀ s1 s2 : atom, {s1 = s2} + {s1 ≠ s2} := string_dec.
+Definition atom_eqb: atom → atom → bool := String.eqb.
+Definition atom_eqb_spec (s1 s2 : atom): reflect (s1 = s2) (atom_eqb s1 s2) := String.eqb_spec s1 s2.
+
+(** Locally Nameless Functions: *)
+
+(** This Stale class gathers all free variables in type context, values, terms,
+  etc. *)
+Class Stale {D} A := stale : A -> D.
+
+Definition fv_of_set (s: aset): atom := fresh_string_of_set "x" s.
+Lemma fv_of_set_fresh (s: aset) : (fv_of_set s) ∉ s.
+Proof.
+  apply fresh_string_of_set_fresh.
+Qed.
+
+#[global]
+Instance atom_stale : @Stale aset atom := singleton.
+Arguments atom_stale /.
+#[global]
+Instance aset_stale : Stale aset := id.
+Arguments aset_stale /.
+
+Notation "x # s" := (x ∉ stale s) (at level 40).
+
+Class Subst V A := subst : atom -> V -> A -> A.
+
+Notation "'{' x ':=' s '}' t" := (subst x s t) (at level 0).
+
+Class Open V A := open : nat -> V -> A -> A.
+
+Notation "'{' k '~>' v '}' e" := (open k v e) (at level 0, k constr).
+
+Notation "e '^^' s" := (open 0 s e) (at level 20).
+
+Class Close A := close : atom -> nat -> A -> A.
+
+Notation "'{' x '<~' k '}' e" := (close x k e) (at level 0, k constr).
+
+Notation "x '\\' e" := (close x 0 e) (at level 20).
+
+Class Lc A := lc : A -> Prop.
+
+Class Typing G E T := has_type : G -> E -> T -> Prop.
+
+Notation "Γ '⊢' e '⋮' T" := (has_type Γ e T) (at level 20, e constr, T constr, Γ constr).
