ListCtx.v
@@ -1,11 +1,10 @@
 From stdpp Require Import mapset.
-From CT Require Import Atom.
-From CT Require Import NamelessTactics.
+From CT Require Import BaseDef.
+From CT Require Import Tactics.
 From Stdlib Require Import Lists.List.
-Import Atom.
-Import Tactics.
-Import NamelessTactics.
+Import BaseDef.
 Import List.
+From Hammer Require Import Tactics.
 
 (** This file defines an ordered type context used in refinement typing. *)
 
@@ -21,32 +20,20 @@ Fixpoint ctxdom {A: Type} (Γ: listctx A) : aset :=
 
 #[global]
 Instance listctx_stale {A:Type} : Stale (listctx A) := ctxdom.
-Arguments listctx_stale /.
+Arguments listctx_stale /. 
 
 Lemma app_one_eq_nil {A: Type}: forall (x: atom) (tau:A) Γ, ~ ([] = Γ ++ [(x, tau)]).
-Proof.
-  intros. intro H. symmetry in H. apply app_eq_nil in H. destruct H. inversion H0.
-Qed.
+Proof. destruct Γ; sauto. Qed.
 
 Lemma app_one_is_cons {A: Type}: forall (x: A) l, (x::nil) ++ l = x :: l.
-Proof. simpl. reflexivity. Qed.
+Proof. hauto. Qed.
 
 Lemma app_list_unit_eq_unit {A: Type}: forall (x y: A) l, l ++ [x] = [y] -> x = y /\ l = [].
-Proof. intros. apply app_eq_unit in H.
-       destruct H.
-       destruct H. inversion H0. split; auto.
-       destruct H. inversion H0.
-Qed.
+Proof. intros. apply app_eq_unit in H. sauto. Qed.
 
-Ltac auto_destruct_pair :=
-  repeat match goal with
-         | [a: prod _ _ |- _] => destruct a
-         end.
-
-Ltac list_app_simpl :=
-  auto_destruct_pair;
-  try auto_exfalso;
-  repeat match goal with
+Ltac list_app_simpl_aux1 :=
+  match goal with
+    | [a: prod _ _ |- _] => destruct a
     | [H: ?Γ1 ++ [(?x1, ?t1)] = ?Γ2 ++ [(?x2, ?t2)] |- _ ] => apply app_inj_tail in H; destruct H; subst
     | [H: (?x1, ?t1) = (?x2, ?t2) |- _ ] => inversion H; subst; clear H
     | [H: context [ ?a ++ []] |- _ ] => rewrite app_nil_r in H
@@ -57,12 +44,16 @@ Ltac list_app_simpl :=
     | [ |- context [(_ :: _) ++ _]] => rewrite <- app_comm_cons
     | [H: context [(_ ++ _) ++ _] |- _ ] => rewrite <- app_assoc in H
     | [ |- context [(_ ++ _) ++ _]] => rewrite <- app_assoc
-    end; auto.
+  end.
+
+Ltac list_app_simpl :=
+  repeat list_app_simpl_aux1; auto.
 
 Lemma ctxdom_app_union {A: Type}: forall (Γ1 Γ2: listctx A), ctxdom (Γ1 ++ Γ2) = (ctxdom Γ1) ∪ (ctxdom Γ2).
 Proof.
-  induction Γ1; simpl; intros; auto. my_set_solver.
-  auto_destruct_pair. rewrite IHΓ1. my_set_solver.
+  induction Γ1; simpl; intros; auto.
+  - set_solver.
+  - list_app_simpl. rewrite IHΓ1. set_solver.
 Qed.
 
 (** Definition of non-duplicate. *)
@@ -75,26 +66,27 @@ Global Hint Constructors ok: core.
 Lemma ok_post_destruct {A: Type}: forall Γ (x: atom) (t: A), ok (Γ ++ [(x, t)]) <-> ok Γ /\ x ∉ ctxdom Γ.
 Proof.
   intros. split.
-  - split; inversion H; subst; repeat list_app_simpl.
-  - intros. destruct H. constructor; auto.
+  - split; inversion H; subst; list_app_simpl;
+    destruct Γ; sauto.
+  - sauto.
 Qed.
 
 Lemma ok_pre_destruct {A: Type}: forall Γ (x: atom) (t: A), ok ((x, t) :: Γ) <-> ok Γ /\ x ∉ ctxdom Γ.
 Proof.
   split; generalize dependent t. generalize dependent x. generalize dependent Γ.
   - apply (rev_ind (fun Γ => forall (x: atom) (t: A), ok ((x, t) :: Γ) -> ok Γ /\ x ∉ ctxdom Γ));
-      simpl; split; intros; auto_destruct_pair; auto; try my_set_solver.
+      simpl; split; intros; list_app_simpl; auto; try set_solver.
     + rewrite app_comm_cons in H0. rewrite ok_post_destruct in H0. destruct H0.
       specialize (H x0 t H0). destruct H.
-      constructor; auto. my_set_solver.
+      constructor; auto. set_solver.
     + rewrite app_comm_cons in H0. rewrite ok_post_destruct in H0. destruct H0.
-      specialize (H x0 t H0). destruct H. rewrite ctxdom_app_union. my_set_solver.
+      specialize (H x0 t H0). destruct H. rewrite ctxdom_app_union. set_solver.
   - apply (rev_ind (fun Γ => forall (x: atom) (t: A), ok Γ /\ x ∉ ctxdom Γ -> ok ((x, t) :: Γ)));
       simpl; intros.
     + destruct H. rewrite <- app_nil_l. constructor; auto.
-    + auto_destruct_pair. destruct H0.
+    + list_app_simpl. destruct H0.
       rewrite ok_post_destruct in H0. destruct H0. rewrite ctxdom_app_union in H1.
-      rewrite app_comm_cons. constructor; auto. apply H; auto. split; auto. my_set_solver. my_set_solver.
+      rewrite app_comm_cons. constructor; auto. apply H; auto. split; auto. set_solver. set_solver.
 Qed.
 
 (** another ok definition *)
@@ -107,30 +99,27 @@ Global Hint Constructors ok_forward: core.
 (** two definitions is equal *)
 Lemma ok_iff_of_ok_forward {A: Type}: forall (Γ: listctx A), ok Γ <-> ok_forward Γ.
 Proof.
-  split.
-  - induction Γ; intros; auto. destruct a. apply ok_pre_destruct in H. destruct H.
-    constructor; auto.
-  - induction Γ; intros; auto. destruct a. rewrite ok_pre_destruct.
-    inversion H; subst. split; auto.
+  split; induction Γ; intros; auto; list_app_simpl.
+  - apply ok_pre_destruct in H. hauto.
+  - rewrite ok_pre_destruct. invert H; hauto.
 Qed.
 
 Lemma ok_weak_pre {A: Type}: forall (Γ1 Γ2: listctx A),
     ok (Γ1 ++ Γ2) -> ok Γ1.
 Proof.
   intros Γ1.
-  apply (rev_ind (fun Γ2 => ok (Γ1 ++ Γ2) -> ok Γ1)); intros.
-  - list_app_simpl.
-  - apply H. rewrite app_assoc in H0. destruct x. rewrite ok_post_destruct in H0.
-    destruct H0; auto.
+  apply (rev_ind (fun Γ2 => ok (Γ1 ++ Γ2) -> ok Γ1)); intros; list_app_simpl.
+  - apply H. 
+    rewrite app_assoc in *.
+    rewrite ok_post_destruct in *. hauto.
 Qed.
 
 Lemma ok_weak_post {A: Type}: forall (Γ2 Γ1: listctx A),
     ok (Γ1 ++ Γ2) -> ok Γ2.
 Proof.
-  intros Γ2. induction Γ1; intros.
-  - list_app_simpl.
-  - apply IHΓ1. rewrite ok_iff_of_ok_forward. rewrite ok_iff_of_ok_forward in H.
-    inversion H; subst. auto.
+  intros Γ2. induction Γ1; intros; list_app_simpl.
+  - apply IHΓ1. rewrite ok_iff_of_ok_forward in *.
+    invert H; hauto.
 Qed.
 
 (** ctxfind *)
@@ -143,33 +132,50 @@ Fixpoint ctxfind {A: Type} (Γ: listctx A) (x: atom): option A :=
 Lemma ctxfind_none_iff_not_in_dom {A: Type}: forall (Γ: listctx A) x,
     ctxfind Γ x = None <-> x ∉ ctxdom Γ.
 Proof with auto.
-  split; generalize dependent x.
-  - induction Γ; simpl; intros; try auto_destruct_pair.
-    + my_set_solver.
-    + var_dec_solver.
-      rewrite decide_True in H; auto; auto_exfalso.
-      rewrite decide_False in H; auto. apply IHΓ in H. my_set_solver.
-  - induction Γ; simpl; intros; try auto_destruct_pair; auto.
-    + var_dec_solver; auto. my_set_solver.
+  split; generalize dependent x; induction Γ; simpl; intros; list_app_simpl.
+  set_solver.
+  all: mydestr; set_solver.
+Qed.
+
+Lemma ctxfind_some_spec1 {A: Type}: forall (Γ: listctx A) x (a: A),
+    ctxfind Γ x = Some a -> ∃ l1 l2, Γ = l1 ++ (x, a) :: l2 /\ x ∉ ctxdom l1.
+Proof.
+  induction Γ; simpl; intros; list_app_simpl.
+  + hauto.
+  + mydestr; auto.
+    - invert H; subst. exists [], Γ. split. hauto. set_solver.
+    - apply IHΓ in H. destruct H as (l1 & l2 & H1 & H2). subst.
+      exists ((a, a1) :: l1), l2. split. hauto. set_solver.
+Qed.
+
+Lemma ctxfind_some_spec2 {A: Type}: forall (Γ: listctx A) x (a: A),
+    (∃ l1 l2, Γ = l1 ++ (x, a) :: l2 /\ x ∉ ctxdom l1) -> ctxfind Γ x = Some a.
+Proof.
+  induction Γ; simpl; intros; list_app_simpl; destruct H as (l1 & l2 & H1 & H2); subst.
+  + destruct l1; hauto.
+  + mydestr; list_app_simpl.
+    - destruct l1. hauto. set_solver.
+    - destruct l1. hauto. set_solver.
+Qed.
+
+Lemma ctxfind_some_spec {A: Type}: forall (Γ: listctx A) x (a: A),
+    ctxfind Γ x = Some a <-> ∃ l1 l2, Γ = l1 ++ (x, a) :: l2 /\ x ∉ ctxdom l1.
+Proof.
+  split. apply ctxfind_some_spec1. apply ctxfind_some_spec2.
 Qed.
 
 Lemma ctxfind_some_implies_in_dom {A: Type}: forall (Γ: listctx A) x (a: A),
     ctxfind Γ x = Some a -> x ∈ ctxdom Γ.
-Proof with auto.
-  induction Γ; simpl; intros; try auto_destruct_pair.
-  + auto_exfalso.
-  + repeat var_dec_solver. set_solver. apply IHΓ in H. my_set_solver.
+Proof.
+  intros. rewrite ctxfind_some_spec in H. destruct H as (l1 & l2 & H1 & H2). subst. rewrite ctxdom_app_union. set_solver.
 Qed.
 
-Ltac listctx_set_simpl' :=
-  list_app_simpl;
-  repeat match goal with
+Ltac listctx_set_simpl_aux :=
+  match goal with
     | [H: ctxfind _ _ = Some _ |- _ ⊆ _ ] => apply ctxfind_some_implies_in_dom in H
     | [H: ctxfind _ _ = Some _ |- _ ∉ _ ] => apply ctxfind_some_implies_in_dom in H
     | [H: ctxfind _ _ = Some _ |- _ ∈ _ ] => apply ctxfind_some_implies_in_dom in H
     | [H: ctxfind _ _ = None |- _ ] => rewrite ctxfind_none_iff_not_in_dom in H
-    | [H: context [ctxdom (_ ++ _)] |- _ ] =>
-        rewrite ctxdom_app_union in H; simpl in H
     | [|- ctxfind _ _ = None ] => rewrite ctxfind_none_iff_not_in_dom
     | [H: ok (((?x, _) :: _) ++ [(?y, _)]) |- _ ] =>
         rewrite <- app_comm_cons in H
@@ -177,40 +183,48 @@ Ltac listctx_set_simpl' :=
         rewrite ok_pre_destruct in H; destruct H
     | [H: ok (_ ++ [(_, _)]) |- _ ] =>
         rewrite ok_post_destruct in H; destruct H
-    | [H: context [ctxdom (_ ++ [(_, _)])] |- _ ] =>
+    | [H: context [ctxdom (_ ++ _)] |- _ ] =>
         rewrite ctxdom_app_union in H; simpl in H
-    | [|- context [ctxdom (_ ++ [(_, _)])]] =>
+    (* | [H: context [ctxdom (_ ++ [(_, _)])] |- _ ] =>
+        rewrite ctxdom_app_union in H; simpl in H *)
+    | [|- context [ctxdom (_ ++ _)] ] =>
         rewrite ctxdom_app_union; simpl
-    | [|- context [ctxdom (_ ++ _)]] =>
-        rewrite ctxdom_app_union; simpl
+    (* | [|- context [ctxdom (_ ++ [(_, _)])]] =>
+        rewrite ctxdom_app_union; simpl *)
+    (* | [|- context [ctxdom (_ ++ _)]] =>
+        rewrite ctxdom_app_union; simpl *)
     end.
+
+Ltac listctx_set_simpl' := 
+  repeat (first [list_app_simpl_aux1 | listctx_set_simpl_aux ]); auto.
 
 Lemma ctxfind_none_neq_hd {A: Type}: forall (Γ: listctx A) x tx a,
     ctxfind ((x, tx):: Γ) a = None -> x <> a.
 Proof with auto.
-  intros. rewrite ctxfind_none_iff_not_in_dom in H. my_set_solver.
+  intros. rewrite ctxfind_none_iff_not_in_dom in H. set_solver.
 Qed.
+
+Ltac ok_list_simpl :=
+  match goal with
+    | [H: ok (_ :: _) |- _ ] => apply ok_pre_destruct in H
+    | [H: ok (_ ++ [_]) |- _ ] => apply ok_post_destruct in H
+  end; auto.
 
 Lemma ctxfind_app {A: Type}: forall Γ1 Γ2 x (T: A),
     ok (Γ1 ++ Γ2) ->
     ctxfind (Γ1 ++ Γ2) x = Some T <-> ctxfind Γ1 x = Some T \/ ctxfind Γ2 x = Some T.
 Proof.
   induction Γ1; split; intros; listctx_set_simpl'.
-  - destruct H0; auto. inversion H0.
-  - destruct (Atom.atom_dec a x); subst; simpl in H0; auto.
-    + left. repeat var_dec_solver.
-    + simpl. repeat var_dec_solver. rewrite <- IHΓ1; auto.
-  - destruct H0; simpl in H0; auto.
-    + repeat var_dec_solver. rewrite IHΓ1; auto.
-    + repeat var_dec_solver. apply ctxfind_some_implies_in_dom in H0. my_set_solver.
-      rewrite IHΓ1; auto.
-Qed.
+  - hauto.
+  - hauto.
+  - simpl in *; mydestr; auto.
+    + intuition. apply ctxfind_some_implies_in_dom in H2. set_solver. 
+    + hauto.
+Qed.  
 
 Lemma ctxfind_app_exclude {A: Type}: forall (Γ1 Γ2: listctx A), ok (Γ1 ++ Γ2) -> (ctxdom Γ1) ∩ (ctxdom Γ2) = ∅.
 Proof.
-  induction Γ1; intros; simpl; listctx_set_simpl'.
-  - fast_set_solver.
-  - my_set_solver.
+  induction Γ1; intros; simpl; listctx_set_simpl'; set_solver.
 Qed.
 
 Lemma ctxfind_app_weaken {A: Type}: forall Γ1 Γ2 Γ3 x (T: A),
@@ -219,23 +233,24 @@ Lemma ctxfind_app_weaken {A: Type}: forall Γ1 Γ2 Γ3 x (T: A),
 Proof.
   induction Γ1; simpl; intros; listctx_set_simpl'.
   - rewrite ctxfind_app; auto.
-  - repeat var_dec_solver.
+  - hauto.
 Qed.
 
 Lemma ok_app_weaken {A: Type}: forall (Γ1 Γ2: listctx A) x (Tx :A),
     ok (Γ1 ++ (x, Tx) :: Γ2) -> ok (Γ1 ++ Γ2).
 Proof.
   induction Γ1; simpl; intros; listctx_set_simpl'; auto.
-  - apply IHΓ1 in H. rewrite ok_pre_destruct. split; auto. listctx_set_simpl'. my_set_solver.
+  - apply IHΓ1 in H. rewrite ok_pre_destruct. listctx_set_simpl'. set_solver.
 Qed.
 
 Lemma ctxfind_find_mid_eq {A: Type}: forall (Γ1 Γ3: listctx A) x (U T:A),
     ok (Γ1 ++ (x, U) :: Γ3) ->
     ctxfind (Γ1 ++ (x, U) :: Γ3) x = Some T -> U = T.
 Proof.
-  induction Γ1; simpl; intros; listctx_set_simpl'; auto.
-  - repeat var_dec_solver.
-  - repeat var_dec_solver. my_set_solver.
+  intros. rewrite ctxfind_app in H0; auto. destruct H0; auto.
+  + apply ctxfind_app_exclude in H. 
+    apply ctxfind_some_implies_in_dom in H0. set_solver.
+  + hauto. 
 Qed.
 
 Lemma ctxfind_find_mid_neq {A: Type}: forall (Γ1 Γ3: listctx A) x y (U T:A),
@@ -243,20 +258,16 @@ Lemma ctxfind_find_mid_neq {A: Type}: forall (Γ1 Γ3: listctx A) x y (U T:A),
     ok (Γ1 ++ (x, U) :: Γ3) ->
     ctxfind (Γ1 ++ (x, U) :: Γ3) y = Some T -> ctxfind (Γ1 ++ Γ3) y = Some T.
 Proof.
-  induction Γ1; simpl; intros; listctx_set_simpl'; auto.
-  - repeat var_dec_solver.
-  - repeat var_dec_solver. my_set_solver.
+  induction Γ1; simpl; intros; listctx_set_simpl'; hauto.
 Qed.
 
 Lemma find_mid_eq_singleton_simp {A: Type} : forall (x1 x2: atom) (τ1 τ2: A) Γ1 Γ2,
     [(x1, τ1)] = Γ1 ++ (x2, τ2) :: Γ2 -> x1 = x2 /\ τ1 = τ2 /\ Γ1 = [] /\ Γ2 = [].
 Proof.
   intros.
-  destruct Γ1; listctx_set_simpl'; invclear H.
-  - repeat split; auto.
-  - listctx_set_simpl'.
+  destruct Γ1; invert H; listctx_set_simpl'.
+  destruct Γ1; hauto.
 Qed.
-
 
 Lemma find_mid_eq_cons_simp {A: Type} : forall (x1 x2: atom) (τ1 τ2: A) Γ1 Γ2 Γ,
     (x1, τ1) :: Γ = Γ1 ++ (x2, τ2) :: Γ2 ->
@@ -264,49 +275,59 @@ Lemma find_mid_eq_cons_simp {A: Type} : forall (x1 x2: atom) (τ1 τ2: A) Γ1 Γ
       (exists Γ1', Γ = Γ1' ++ (x2, τ2) ::  Γ2 /\ Γ1 = (x1, τ1) :: Γ1').
 Proof.
   intros.
-  destruct Γ1; invclear H.
-  - left. repeat split; auto.
-  - right. exists Γ1. repeat split; auto.
+  destruct Γ1; (invert H; listctx_set_simpl'); hauto.
 Qed.
 
-Ltac listctx_set_simpl1 :=
-  list_app_simpl;
-  repeat (listctx_set_simpl' ||
-            (match goal with
-             | [H: context [ctxfind [] _] |- _ ] => progress simpl in H
-             | [|- context [ctxfind [] _]] => progress simpl
-             | [H1: ok (?Γ1 ++ (?x, ?U) :: ?Γ3), H: ctxfind (?Γ1 ++ (?x, ?U) :: ?Γ3) ?x = Some ?T |- _ ] => assert (U = T) as Htmp by (apply (ctxfind_find_mid_eq _ _ _ _ T) in H1; auto); subst; try clear Htmp
-             | [H: ctxfind (?Γ1 ++ (?z, _) :: ?Γ3) ?x = Some ?T
-                |- ctxfind (?Γ1 ++ ?Γ3) ?x = Some ?T ] => apply ctxfind_find_mid_neq in H; auto
-| [H: (_, _) :: _ = (_, _):: _ |- _ ] => invclear H
-            | [H: [(_, _)] = _ ++ (_, _) :: _ |- _ ] => apply find_mid_eq_singleton_simp in H; mydestr; subst
-            | [H: (_, _) :: _ = _ ++ (_, _) :: _ |- _ ] => apply find_mid_eq_cons_simp in H; destruct H; mydestr; subst
-             end)).
-
-Ltac listctx_set_simpl2 :=
-  repeat (listctx_set_simpl1 ||
-            match goal with
-            | [H: (_, _) :: _ = (_, _):: _ |- _ ] => invclear H
-            | [H: [(_, _)] = _ ++ (_, _) :: _ |- _ ] => apply find_mid_eq_singleton_simp in H; mydestr; subst
-            | [H: (_, _) :: _ = _ ++ (_, _) :: _ |- _ ] => apply find_mid_eq_cons_simp in H; destruct H; mydestr; subst
-            end).
-
-Ltac listctx_set_simpl3 :=
+Ltac listctx_set_simpl_aux2 :=
   match goal with
-  | [H: _ ++ [_] = [_] |- _ ] => apply elt_eq_unit in H; mydestr; subst
-  | [H: _ ++ [_] = _ :: _ ++ [_] |- _ ] => rewrite app_comm_cons in H; listctx_set_simpl2
-  end || listctx_set_simpl2.
-
-Ltac listctx_set_simpl4 :=
-  match goal with
+  | [H: context [ctxfind [] _] |- _ ] => progress simpl in H
+  | [|- context [ctxfind [] _]] => progress simpl
+  | [H1: ok (?Γ1 ++ (?x, ?U) :: ?Γ3), H: ctxfind (?Γ1 ++ (?x, ?U) :: ?Γ3) ?x = Some ?T |- _ ] => 
+    assert (U = T) as Htmp by (apply (ctxfind_find_mid_eq _ _ _ _ T) in H1; auto); subst; try clear Htmp
+  | [H: ctxfind (?Γ1 ++ (?z, _) :: ?Γ3) ?x = Some ?T
+ |- ctxfind (?Γ1 ++ ?Γ3) ?x = Some ?T ] => 
+    apply ctxfind_find_mid_neq in H
+  | [H: (_, _) :: _ = (_, _):: _ |- _ ] => invclear H
+  | [H: [(_, _)] = _ ++ (_, _) :: _ |- _ ] => 
+    apply find_mid_eq_singleton_simp in H; subst
+  | [H: (_, _) :: _ = _ ++ (_, _) :: _ |- _ ] => 
+    apply find_mid_eq_cons_simp in H; destruct H; subst
+  | [H: (_, _) :: _ = (_, _):: _ |- _ ] => invclear H
+  | [H: [(_, _)] = _ ++ (_, _) :: _ |- _ ] => 
+    apply find_mid_eq_singleton_simp in H; subst
+  | [H: (_, _) :: _ = _ ++ (_, _) :: _ |- _ ] => 
+    apply find_mid_eq_cons_simp in H; destruct H; subst
+  | [H: _ ++ [_] = [_] |- _ ] => apply elt_eq_unit in H; subst
+  | [H: _ ++ [_] = _ :: _ ++ [_] |- _ ] => rewrite app_comm_cons in H
   | [H: _ ++ [_] = _ ++ _ ++ [_] |- _ ] =>
-      rewrite app_assoc in H;
-      apply app_inj_tail in H; mydestr; subst; listctx_set_simpl3
-  end || listctx_set_simpl3.
+    rewrite app_assoc in H;
+    apply app_inj_tail in H; subst
+end.
 
-Ltac listctx_set_simpl := listctx_set_simpl4.
+Ltac listctx_set_simpl := 
+  repeat (first [list_app_simpl_aux1 | listctx_set_simpl_aux | listctx_set_simpl_aux2 ]; auto).
+
+Ltac listctx_set_solver_aux1 :=
+  match goal with
+    | [|- _ <> _] => fast_set_solver !!
+    | [|- _ = _] => fast_set_solver !!
+    | [|- _ ∉ _] => fast_set_solver !!
+    | [|- _ ∈ _] => fast_set_solver !!
+    | [|- _ ⊆ _] => fast_set_solver !!
+    | [H: ctxfind (?Γ1 ++ ?Γ3) ?x = Some ?T |- ctxfind (?Γ1 ++ ?Γ2 ++ ?Γ3) ?x = Some ?T ] => apply ctxfind_app_weaken; auto
+    | [H: ok (?Γ1 ++ _ :: ?Γ2) |- ok (?Γ1 ++ ?Γ2) ] => apply ok_app_weaken in H; exact H
+    | [H: ok (_ ++ (?x, _) :: ?Γ) |- ?x ∉ ctxdom ?Γ ] =>
+        apply ok_weak_post in H; rewrite ok_pre_destruct in H; destruct H; auto
+    | [H: ok (?a ++ ?b ++ ?c) |- ok ((?a ++ ?b) ++ ?c) ] => rewrite <- app_assoc; exact H
+    | [H: ok (?a ++ ?b ++ ?c) |- ok (?a ++ ?b ++ ?c ++ [(?x, _)]) ] =>
+        rewrite -> app_assoc; rewrite -> app_assoc; constructor
+    | [|- ok ((_, _) :: _) ] => rewrite ok_pre_destruct; split; auto
+  end.
 
 Ltac listctx_set_solver1 :=
+  listctx_set_simpl; listctx_set_solver_aux1; fast_set_solver !!.
+
+(* Ltac listctx_set_solver1 :=
   repeat (listctx_set_simpl;
           match goal with
           | [|- _ <> _] => fast_set_solver !!
@@ -322,7 +343,7 @@ Ltac listctx_set_solver1 :=
           | [H: ok (?a ++ ?b ++ ?c) |- ok (?a ++ ?b ++ ?c ++ [(?x, _)]) ] =>
               rewrite -> app_assoc; rewrite -> app_assoc; constructor
           | [|- ok ((_, _) :: _) ] => rewrite ok_pre_destruct; split; auto
-          end); listctx_set_simpl; fast_set_solver !!.
+          end); listctx_set_simpl; fast_set_solver !!. *)
 
 Lemma ctxfind_none_neq_tl {A: Type}: forall (Γ: listctx A) x tx a,
     ctxfind ((x, tx):: Γ) a = None -> ctxfind Γ a = None.
@@ -345,10 +366,7 @@ Proof. intros; listctx_set_solver1. Qed.
 Lemma l_find_implies_in {A:Type}: forall (ctx: listctx A) (x: atom) (t: A),
       ctxfind ctx x = Some t -> In (x, t) ctx.
 Proof.
-  induction ctx; simpl; intros; listctx_set_simpl.
-  var_dec_solver.
-  + left. var_dec_solver; auto_eq_post.
-  + right. var_dec_solver.
+  induction ctx; simpl; intros; listctx_set_simpl; hauto.
 Qed.
 
 Lemma ctxfind_some_spec_aux {A:Type}: forall (ctx: list (prod atom A)) (name: atom) (tau: A),
@@ -378,26 +396,28 @@ Ltac auto_exfalso_ok :=
     end;
   auto_exfalso.
 
+Ltac listctx_set_solver_aux2 :=
+  match goal with
+  | [H: ok ?Γ |- ok [(?x, _); (?y, _)]] => 
+    rewrite <- app_one_is_cons; constructor; auto
+  | [H: ok ?Γ |- ok (?Γ ++ [(?x, _); (?y, _)])] => 
+    rewrite <- app_one_is_cons in H; rewrite app_assoc in H; constructor; auto
+  | [H: ok ?Γ |- ok (?Γ ++ [(?x, _)])] => econstructor; eauto
+  end.
+
 Ltac listctx_set_solver2 :=
-  repeat match goal with
-    | [H: ok ?Γ |- ok [(?x, _); (?y, _)]] => rewrite <- app_one_is_cons; constructor; auto
-    | [H: ok ?Γ |- ok (?Γ ++ [(?x, _); (?y, _)])] => rewrite <- app_one_is_cons; rewrite app_assoc; constructor; auto
-    | [H: ok ?Γ |- ok (?Γ ++ [(?x, _)])] => econstructor; eauto
-    end; auto;
-  (auto_exfalso_ok || listctx_set_solver1).
+  listctx_set_simpl;
+  repeat (first [listctx_set_solver_aux2 | listctx_set_solver_aux1]; auto);
+  (auto_exfalso_ok || fast_set_solver !!).
 
 Lemma ctxfind_last_eq {A:Type}: forall (ctx: list (prod atom A)) name tau,
     ok (ctx ++ [(name, tau)]) ->
     ctxfind (ctx ++ [(name, tau)]) name = Some tau.
 Proof with eauto.
   induction ctx; intros; listctx_set_simpl.
-  - repeat var_dec_solver.
-  - simpl. rewrite decide_False. apply IHctx. constructor; auto. my_set_solver.
+  - hauto.
+  - simpl. mydestr. set_solver. hauto. 
 Qed.
-
-Ltac var_dec_solver_exfalso :=
-  var_dec_solver;
-  try auto_exfalso_ok.
 
 Lemma ctxfind_last_neq_none {A:Type}: forall (ctx: list (prod atom A)) name tau a,
     name <> a ->
@@ -410,39 +430,27 @@ Lemma ctxfind_last_neq {A:Type}: forall (ctx: list (prod atom A)) name tau a tau
     name <> a ->
     ctxfind (ctx ++ [(name, tau)]) a = Some tau_a <->
       ctxfind ctx a = Some tau_a.
-Proof with eauto.
-  intros. induction ctx...
-  - simpl. split; intros; repeat var_dec_solver_exfalso.
-  - try auto_destruct_pair.
-    listctx_set_simpl.
-    simpl. split; intros; repeat var_dec_solver_exfalso.
-    apply IHctx in H3; auto. rewrite IHctx; auto.
-Qed.
-
-Lemma ctxfind_some_spec {A:Type}: forall (ctx: list (prod atom A)) (name: atom) (tau: A),
-    ok ctx ->
-    ctxfind ctx name = Some tau ->
-    (exists ctx1 ctx2,
-        ctx = ctx1 ++ [(name, tau)] ++ ctx2 /\ ctxfind ctx2 name = None
-    ).
 Proof.
-  intros.
-  apply ctxfind_some_spec_aux in H0.
-  destruct H0 as (Γ1 & Γ2 & Happ). exists Γ1, Γ2. split; auto.
-  rewrite Happ in H. listctx_set_solver2.
+  intros. induction ctx; listctx_set_simpl; hauto. 
 Qed.
 
 Lemma find_none_append {A: Type}: forall Γ a (tau_x: A) x,
     ctxfind Γ a = None ->
     x <> a ->
     ctxfind (Γ ++ ((x,tau_x)::nil)) a = None.
-Proof with eauto.
+Proof.
   intros. listctx_set_solver2.
 Qed.
 
-Ltac listctx_set_solver3 :=
-  simpl;
-  repeat match goal with
+Lemma ok_single {A: Type}: forall (x: atom) (T: A), ok [(x, T)].
+Proof.
+  intros.
+  rewrite ok_pre_destruct; split; auto; fast_set_solver.
+Qed.
+
+Ltac listctx_set_solver_aux3 :=
+  match goal with
+    | [|- ok [(_, _)]] => apply ok_single
     | [H: ok (_ ++ ?Γ) |- ok ?Γ] => apply ok_weak_post in H; auto
     | [H: ok (?Γ ++ _) |- ok ?Γ] => apply ok_weak_pre in H; auto
     | [|- _ ∉ _ ] => listctx_set_solver2
@@ -459,64 +467,62 @@ Ltac listctx_set_solver3 :=
         rewrite <- app_one_is_cons;
         rewrite app_assoc; rewrite <- (app_one_is_cons (x, T));
         rewrite app_assoc; constructor; auto
-    end; auto;
-  listctx_set_solver2.
+  end.
 
-Lemma ok_single {A: Type}: forall (x: atom) (T: A), ok [(x, T)].
-Proof.
-  intros.
-  rewrite ok_pre_destruct; split; auto; fast_set_solver.
-Qed.
-
-Ltac listctx_set_solver4 :=
-  match goal with
-  | [|- ok [(_, _)]] => apply ok_single
-  end || listctx_set_solver3.
+Ltac listctx_set_solver3 :=
+  listctx_set_simpl;
+  repeat (first [listctx_set_solver_aux3; listctx_set_solver_aux2 | listctx_set_solver_aux1]; auto);
+  (auto || auto_exfalso_ok || fast_set_solver !!).
 
 Lemma ctxfind_in {A: Type}: forall Γv1 (x: atom) (u: A) Γv2,
     ok (Γv1 ++ (x, u) :: Γv2) ->
     ctxfind (Γv1 ++ (x, u) :: Γv2) x = Some u.
 Proof.
-  induction Γv1; simpl; intros; mydestr; auto.
-  - repeat var_dec_solver.
-  - repeat var_dec_solver; listctx_set_solver4.
+  induction Γv1; simpl; intros; mydestr; auto; listctx_set_simpl.
+  - hauto.
+  - set_solver.
 Qed.
 
 Lemma ok_mid_insert {A: Type} : forall Γ1 (x: atom) (T: A) Γ2,
     (x ∉ ctxdom Γ1 ∪ ctxdom Γ2 /\ ok (Γ1 ++ Γ2)) <-> ok (Γ1 ++ (x, T) :: Γ2).
 Proof.
-  induction Γ1; split; simpl; intros; mydestr; repeat split; auto; try listctx_set_solver4.
+  induction Γ1; split; simpl; intros; mydestr; repeat split; auto; try listctx_set_solver3.
   - rewrite ok_pre_destruct. split.
-    + apply IHΓ1; repeat split; listctx_set_solver4.
-    + listctx_set_solver4.
-  - rewrite ok_pre_destruct in H; mydestr. rewrite <- IHΓ1 in H; mydestr. listctx_set_solver4.
+    + apply IHΓ1; repeat split; listctx_set_solver3.
+    + listctx_set_solver3.
+  - rewrite ok_pre_destruct in H; mydestr. rewrite <- IHΓ1 in H; mydestr. listctx_set_solver3.
 Qed.
 
 Lemma ok_app_swap {A: Type} : forall (Γ1: listctx A) Γ2, ok (Γ1 ++ Γ2) <-> ok (Γ2 ++ Γ1).
 Proof.
-  induction Γ1; split; simpl; intros; mydestr; try listctx_set_solver4.
+  induction Γ1; split; simpl; intros; mydestr; try listctx_set_solver3.
   - rewrite ok_pre_destruct in H; mydestr. rewrite IHΓ1 in H.
-    rewrite <- ok_mid_insert; split; listctx_set_solver4.
+    rewrite <- ok_mid_insert; split; listctx_set_solver3.
   - rewrite <- ok_mid_insert in H; mydestr. rewrite <- IHΓ1 in H0.
-    rewrite ok_pre_destruct; split; auto; listctx_set_solver4.
+    rewrite ok_pre_destruct; split; auto; listctx_set_solver3.
 Qed.
 
 Lemma ok_app_swap3 {A: Type} : forall (Γ1: listctx A) Γ2 Γ3, ok (Γ1 ++ Γ2 ++ Γ3) <-> ok (Γ2 ++ Γ1 ++ Γ3).
 Proof.
-  induction Γ1; split; simpl; intros; mydestr; try listctx_set_solver4.
+  induction Γ1; split; simpl; intros; mydestr; try listctx_set_solver3; auto.
   - rewrite ok_pre_destruct in H; mydestr. rewrite IHΓ1 in H.
-    rewrite <- ok_mid_insert; split; listctx_set_solver4.
+    rewrite <- ok_mid_insert; split; listctx_set_solver3.
   - rewrite <- ok_mid_insert in H; mydestr. rewrite <- IHΓ1 in H0.
-    rewrite ok_pre_destruct; split; auto; listctx_set_solver4.
+    rewrite ok_pre_destruct; split; auto; listctx_set_solver3.
 Qed.
 
-Ltac listctx_set_solver5 :=
+Ltac listctx_set_solver_aux5 :=
   match goal with
   | [H: ok (?a ++ ?b) |- ok (?b ++ ?a)] => rewrite ok_app_swap; auto
   | [H: ok (?a ++ ?b ++ ?c) |- ok (?b ++ ?a ++ ?c)] => rewrite ok_app_swap3; auto
   | [H: ok (?Γ1 ++ ?Γ2 ++ ?Γ3) |- ok (?Γ1 ++ ?Γ3)] =>
-         rewrite ok_app_swap3 in H; listctx_set_solver4
-  end || listctx_set_solver4.
+         rewrite ok_app_swap3 in H; listctx_set_solver3
+  end.
+
+Ltac listctx_set_solver5 :=
+  listctx_set_simpl;
+  repeat (first [listctx_set_solver_aux5; listctx_set_solver_aux3; listctx_set_solver_aux2 | listctx_set_solver_aux1]; auto);
+  (auto || auto_exfalso_ok || fast_set_solver !!).
 
 Ltac listctx_set_solver := listctx_set_solver5.
 
@@ -525,9 +531,8 @@ Lemma ok_find_same {A: Type}: forall (a: atom) (τ1 τ2: A) Γ1 Γ2 Γ1' Γ2',
     Γ1 = Γ1' /\ τ1 = τ2 /\ Γ2 = Γ2'.
 Proof.
   intros a τ1 τ2.
-  induction Γ1; intros; listctx_set_simpl2.
-  apply IHΓ1 in H0; auto. mydestr; subst.
-  repeat split; auto.
+  induction Γ1; intros; mydestr; listctx_set_simpl; mydestr; subst; try listctx_set_solver3.
+  apply IHΓ1 in H0; auto. mydestr; subst. hauto.
 Qed.
 
 Lemma ok_find_neq_head {A: Type}: forall (x a: atom) (τ_x τ_a: A) Γ1' Γ2 Γ2',
@@ -536,6 +541,5 @@ Lemma ok_find_neq_head {A: Type}: forall (x a: atom) (τ_x τ_a: A) Γ1' Γ2 Γ2
     (exists Γ1'', Γ1' = (x, τ_x) :: Γ1'' /\ Γ2 = (Γ1'' ++ (a, τ_a) :: Γ2')).
 Proof.
   intros x a τ_x τ_a Γ1'.
-  induction Γ1'; intros; listctx_set_simpl2.
-  exists Γ1'. split; auto.
+  induction Γ1'; intros; listctx_set_simpl; hauto.
 Qed.
