Syntax/Primitives.v
@@ -1,0 +1,54 @@
+(** * This file defines the primitives of the core language. *)
+Inductive constant : Type :=
+| cbool: bool -> constant
+| cnat : nat -> constant.
+
+Global Hint Constructors constant: core.
+
+(** * basic types *)
+Inductive base_ty : Type :=
+| TNat   : base_ty
+| TBool  : base_ty.
+
+Global Hint Constructors base_ty: core.
+
+Inductive ty : Type :=
+| TBase : base_ty -> ty
+| TArrow : ty -> ty -> ty.
+
+Global Hint Constructors ty: core.
+
+Coercion TBase : base_ty >-> ty.
+Coercion cbool : bool >-> constant.
+Coercion cnat : nat >-> constant.
+
+(* notation for function type: \rightbkarrow. *)
+Notation " t1 '⤍' t2" := (TArrow t1 t2) (at level 18, right associativity).
+
+(** * effectful operators (op in Fig. 4) *)
+(** pure operators (e.g., [op_plus_one]) are treated as effectful operators,
+  whose return value is independent of the context trace, and will not interfere
+  the result of other operators. *)
+Inductive effop : Type :=
+| op_plus_one
+| op_eq_zero
+| op_rannat.
+
+Global Hint Constructors effop: core.
+
+(** This file defines the basic type system of λᴱ. *)
+
+Definition ty_of_const (c: constant): base_ty :=
+  match c with
+  | cnat _ => TNat
+  | cbool _ => TBool
+  end.
+
+Definition ret_ty_of_op (op: effop): base_ty :=
+  match op with
+  | op_plus_one => TNat
+  | op_eq_zero => TBool
+  | op_rannat => TNat
+  end.
+
+Definition ty_of_op (op: effop): ty := TNat ⤍ (ret_ty_of_op op).
