Syntax/Qualifier.v
@@ -1,0 +1,174 @@
+From stdpp Require Import mapset.
+From stdpp Require Import natmap.
+From stdpp Require Import fin vector.
+From CT Require Import BaseDef.
+From CT Require Import Syntax.Primitives.
+From CT Require Import Syntax.Lang.
+
+Import BaseDef.
+Import Primitives.
+Import Lang.
+
+(** This file defines the qualifiers used in refinement types, corresponding to
+  ϕ in Fig. 4. In contrast to the syntactic presentation in paper, propositions
+  are encoded as shallowly embedded Coq propositions. *)
+
+(** A qualifier is defined as a Coq proposition [prop], with closed arguments
+  corresponding to the possibly open [vals]. [vals] captures the variables that
+  are referred to in [prop]. We use length-indexed list [vec] to make sure
+  [prop] arguments and [vals] match exactly. *)
+Inductive qualifier : Type :=
+| qual {n : nat} (vals : vec value n) (prop : vec constant n -> Prop).
+
+(** For example, a qualifier may be: (with notation from stdpp)
+<<
+qual [# vbvar 0; vbvar 1; vfvar "x"]
+   (fun v => v !!! 0 = v !!! 1 /\ v !!! 2 = cnat 1)%fin
+>>
+
+It means the first and second bound variables are equal, and the free variable
+[x] is [1].
+*)
+
+(** Conjunction of two qualifiers *)
+Definition qualifier_and (q1 q2 : qualifier) : qualifier :=
+  match q1, q2 with
+  | qual vals1 prop1, qual vals2 prop2 =>
+      qual (vals1 +++ vals2)
+        (fun v =>
+           let (v1, v2) := Vector.splitat _ v
+           in prop1 v1 /\ prop2 v2)
+  end.
+
+(** * Qualifier denotation *)
+
+Fixpoint denote_vals {n} (vals : vec value n) : option (vec constant n) :=
+  match vals with
+  | [#] => Some [#]
+  | x ::: v =>
+      match x with
+      | vconst c =>
+          match denote_vals v with
+          | Some v' => Some (c ::: v')
+          | None => None
+          end
+      | _ => None
+      end
+  end.
+
+(** Denote a _closed_ qualifier to a Coq proposition. The result is [False] if the
+qualifier mentions functions. *)
+Definition denote_qualifier (ϕ : qualifier) : Prop :=
+  match ϕ with
+  | qual vals prop =>
+      match denote_vals vals with
+      | Some v => prop v
+      | None => False
+      end
+  end.
+
+(** * Notations *)
+
+Definition mk_q_bvar_eq_val n v :=
+  qual [# vbvar n; v] (fun v => v !!! 0 = v !!! 1)%fin.
+Definition mk_q_under_bot := qual [#] (fun _ => False).
+Definition mk_q_under_top := qual [#] (fun _ => True).
+
+Notation " 'b0:v=' v " := (mk_q_bvar_eq_val 0 v)
+                            (at level 5, format "b0:v= v", v constr).
+Notation " 'b0:x=' y " := (mk_q_bvar_eq_val 0 (vfvar y))
+                            (at level 5, format "b0:x= y", y constr).
+Notation " 'b0:c=' c " := (mk_q_bvar_eq_val 0 (vconst c))
+                            (at level 5, format "b0:c= c", c constr).
+Notation " 'b1:v=' v " := (mk_q_bvar_eq_val 1 v)
+                            (at level 5, format "b1:v= v", v constr).
+Notation " 'b1:x=' y " := (mk_q_bvar_eq_val 1 (vfvar y))
+                            (at level 5, format "b1:x= y", y constr).
+Notation " 'b1:c=' c " := (mk_q_bvar_eq_val 1 (vconst c))
+                            (at level 5, format "b1:c= c", c constr).
+Notation " ϕ1 '&' ϕ2 " := (qualifier_and ϕ1 ϕ2)
+                             (at level 5, format "ϕ1  &  ϕ2").
+
+(** * Naming related definitions and lemmas *)
+
+(** free variables *)
+Definition qualifier_fv ϕ : aset :=
+  match ϕ with
+  | qual vals _ => Vector.fold_right (fun v s => fv_value v ∪ s) vals ∅
+  end.
+
+#[global]
+Instance qualifier_stale : @Stale aset qualifier := qualifier_fv.
+Arguments qualifier_stale /.
+
+Definition qualifier_open (k: nat) (s: value) (ϕ: qualifier) : qualifier :=
+  match ϕ with
+  | qual vals prop =>
+      qual (vmap (open_value k s) vals) prop
+  end.
+
+#[global]
+Instance open_qualifier_with_value : Open value qualifier := qualifier_open.
+Arguments open_qualifier_with_value /.
+
+(* Opening values/terms with an atom binder (used in [lc] definitions) *)
+#[global]
+Instance open_qualifier_with_atom : Open atom qualifier :=
+  fun k (a : atom) (ϕ : qualifier) => qualifier_open k (vfvar a) ϕ.
+Arguments open_qualifier_with_atom /.
+
+Definition qualifier_subst (x: atom) (v: value) (ϕ: qualifier) : qualifier :=
+  match ϕ with
+  | qual vals prop =>
+      qual (vmap (value_subst x v) vals) prop
+  end.
+
+#[global]
+Instance subst_qualifier_with_value : Subst value qualifier := qualifier_subst.
+Arguments subst_qualifier_with_value /.
+
+Inductive lc_qualifier : qualifier -> Prop :=
+| lc_qual n vals prop :
+  Vector.Forall (fun v => lc (treturn v)) vals ->
+  lc_qualifier (@qual n vals prop)
+.
+
+Global Hint Constructors lc_qualifier: core.
+
+#[global]
+Instance locally_closed_qualifier_instance : Lc qualifier := lc_qualifier.
+Arguments locally_closed_qualifier_instance /.
+
+(** * Well-founded relation in qualifiers *)
+
+Notation " 'b0≺b1'" :=
+  (qual [# vbvar 0; vbvar 1] (fun v => (v !!! 0) ≺ (v !!! 1))%fin)
+    (at level 5).
+
+Notation " 'b0:x≺' x " :=
+  (qual [# vbvar 0; vfvar x] (fun v => (v !!! 0) ≺ (v !!! 1))%fin)
+    (at level 5, x constr).
+
+Notation " 'b0:v≺' v " :=
+  (qual [# vbvar 0; v] (fun v => (v !!! 0) ≺ (v !!! 1))%fin)
+    (at level 5).
+
+Notation " 'b0:c≺' c " :=
+  (qual [# vbvar 0; vconst c] (fun v => (v !!! 0) ≺ (v !!! 1))%fin)
+    (at level 5).
+
+(** Aux *)
+
+Definition lc_phi1 (ϕ: qualifier) :=
+  exists (L : aset), (forall x : atom, x ∉ L -> lc (ϕ ^^ x)).
+
+Definition lc_phi2 (ϕ: qualifier) :=
+  exists (L : aset), (forall (x : atom), x ∉ L -> forall (y : atom), y ∉ L -> lc ({0 ~> y} ({1 ~> x} ϕ))).
+
+Inductive closed_phi1 (L: aset) (ϕ: qualifier): Prop :=
+| closed_phi_1: stale ϕ ⊆ L -> lc_phi1 ϕ -> closed_phi1 L ϕ.
+  
+Inductive closed_phi2 (L: aset) (ϕ: qualifier): Prop :=
+| closed_phi_2: stale ϕ ⊆ L -> lc_phi2 ϕ -> closed_phi2 L ϕ.
+
+Notation "'⟦' ϕ '⟧q' " := (denote_qualifier ϕ) (at level 20, format "⟦ ϕ ⟧q", ϕ constr).
