Syntax/RefinementType.v
@@ -1,0 +1,190 @@
+Require Import Stdlib.Program.Wf.
+From stdpp Require Import mapset.
+From stdpp Require Import natmap.
+From CT Require Import ListCtx.
+From CT Require Import Syntax.Qualifier.
+
+Import BaseDef.
+Import Lang.
+Import Tactics.
+Import Primitives.
+(* Import OperationalSemantics. *)
+(* Import BasicTyping. *)
+Import Qualifier.
+Import ListCtx.
+Import List.
+
+(** Refinement types (t in Fig. 4) *)
+Inductive rty : Type :=
+| rtyOver (b: base_ty) (ϕ: qualifier)
+| rtyUnder (b: base_ty) (ϕ: qualifier)
+| rtyArr (ρ: rty) (τ: rty).
+
+Global Hint Constructors rty: core.
+
+Notation "'{:' b '|' ϕ '}'" := (rtyOver b ϕ) (at level 5, format "{: b | ϕ }", b constr, ϕ constr).
+Notation "'[:' b '|' ϕ ']' " := (rtyUnder b ϕ) (at level 5, format "[: b | ϕ ]", b constr, ϕ constr).
+Notation "ρ '⇨' τ" :=
+  (rtyArr ρ τ) (at level 80, format "ρ ⇨ τ", right associativity, ρ constr, τ constr).
+
+(* NOTE: \rightwhitearrow: ⇨ *)
+
+Definition is_under_base_rty (τ: rty) :=
+  match τ with
+  | [: _ | _ ] => False
+  | _ => True
+  end.
+
+Definition is_over_base_rty (τ: rty) :=
+  match τ with
+  | {: _ | _ } => False
+  | _ => True
+  end.
+
+(* This measure function is used to guarantee termination of the denotation.
+Instead of addtion, we can also use [max] for the subterms. *)
+Fixpoint rty_measure (ρ: rty) : nat :=
+  match ρ with
+  | rtyOver _ _ | rtyUnder _ _ => 1
+  | ρ ⇨ τ => 1 + rty_measure ρ + rty_measure τ
+  end.
+
+Inductive is_coverage_rty: rty -> Prop :=
+| is_coverage_rty_base: forall b ϕ, is_coverage_rty [:b|ϕ]
+| is_coverage_rty_over_arr: forall b ϕ τ,
+    is_coverage_rty τ -> is_coverage_rty ({:b|ϕ} ⇨ τ)
+| is_coverage_rty_under_arr: forall b ϕ τ,
+    is_coverage_rty τ -> is_coverage_rty ([:b|ϕ] ⇨ τ)
+| is_coverage_rty_arr_arr: forall ρ1 ρ2 τ,
+    is_coverage_rty (ρ1 ⇨ ρ2) -> is_coverage_rty τ -> is_coverage_rty ((ρ1 ⇨ ρ2) ⇨ τ).
+
+Global Hint Constructors is_coverage_rty: core.
+
+Definition fine_rty (τ: rty) :=
+  match τ with
+  | {: _ | _ } => True
+  | [: _ | _ ] => True
+  | _ => is_coverage_rty τ
+  end.
+
+Definition flip_rty (τ: rty) :=
+  match τ with
+  | [: b | ϕ ] => {: b | ϕ }
+  | {: b | ϕ } => [: b | ϕ ]
+  | ρ ⇨ τ => ρ ⇨ τ
+  end.
+
+(** Type erasure (Fig. 5) *)
+
+Fixpoint rty_erase ρ : ty :=
+  match ρ with
+  | {: b | ϕ } => b
+  | [: b | ϕ ] => b
+  | ρ ⇨ τ => (rty_erase ρ) ⤍ (rty_erase τ)
+  end.
+
+Notation " '⌊' ty '⌋' " := (rty_erase ty) (at level 5, format "⌊ ty ⌋", ty constr).
+
+Definition ctx_erase (Γ: listctx rty) :=
+  ⋃ ((List.map (fun e => {[e.1 := rty_erase e.2]}) Γ): list (amap ty)).
+
+Notation " '⌊' Γ '⌋*' " := (ctx_erase Γ) (at level 5, format "⌊ Γ ⌋*", Γ constr).
+
+(** * Naming related definitions *)
+
+Fixpoint rty_fv ρ : aset :=
+  match ρ with
+  | {: _ | ϕ } => qualifier_fv ϕ
+  | [: _ | ϕ ] => qualifier_fv ϕ
+  | ρ ⇨ τ => rty_fv ρ ∪ rty_fv τ
+  end.
+
+#[global]
+  Instance rty_stale : @Stale aset rty := rty_fv.
+Arguments rty_stale /.
+
+Fixpoint open_rty (k: nat) (s: value) (ρ: rty) : rty :=
+  match ρ with
+  | {: b | ϕ } => {: b | qualifier_open (S k) s ϕ }
+  | [: b | ϕ ] => [: b | qualifier_open (S k) s ϕ ]
+  | ρ ⇨ τ => (open_rty k s ρ) ⇨ (open_rty (S k) s τ)
+  end.
+
+#[global]
+Instance open_rty_with_value : Open value rty := open_rty.
+Arguments open_rty_with_value /.
+
+#[global]
+Instance open_rty_with_atom : Open atom rty :=
+  fun k (a : atom) (ρ : rty) => open_rty k (vfvar a) ρ.
+Arguments open_rty_with_atom /.
+
+Fixpoint rty_subst (k: atom) (s: value) (ρ: rty) : rty :=
+  match ρ with
+  | {: b | ϕ} => {: b | qualifier_subst k s ϕ}
+  | [: b | ϕ] => [: b | qualifier_subst k s ϕ]
+  | ρ ⇨ τ => (rty_subst k s ρ) ⇨ (rty_subst k s τ)
+  end.
+
+#[global]
+Instance subst_rty_with_value : Subst value rty := rty_subst.
+Arguments subst_rty_with_value /.
+
+#[global]
+Instance subst_rty_with_atom : Subst atom rty :=
+  fun k (a : atom) (ρ : rty) => rty_subst k (vfvar a) ρ.
+Arguments subst_rty_with_atom /.
+
+(** Local closure *)
+(** NOTE: To alaign with denotation, we assume the function type doesn't appear in transduce. *)
+(** NOTE: all (L: aset) should be the first hypothesis. *)
+Inductive lc_rty : rty -> Prop :=
+| lc_rtyOver: forall b ϕ, lc_phi1 ϕ -> fine_rty {: b | ϕ} -> lc_rty {: b | ϕ}
+| lc_rtyUnder: forall b ϕ, lc_phi1 ϕ -> fine_rty [: b | ϕ] -> lc_rty [: b | ϕ]
+| lc_rtyArr: forall ρ τ (L : aset),
+    (forall x : atom, x ∉ L -> lc_rty (τ ^^ x)) ->
+    fine_rty (ρ ⇨ τ) -> lc_rty ρ ->
+    lc_rty (ρ ⇨ τ).
+
+Global Hint Constructors lc_rty: core.
+
+#[global]
+Instance locally_closed_rty_instance : Lc rty := lc_rty.
+Arguments locally_closed_rty_instance /.
+    
+Lemma lc_rty_fine: forall τ, lc_rty τ -> fine_rty τ.
+Proof.
+  induction 1; eauto.
+Qed.
+
+Definition body_rty τ := exists (L: aset), ∀ x : atom, x ∉ L → lc_rty (τ ^^ x).
+
+(** Closed under free variable set *)
+
+Inductive closed_rty (d : aset) (ρ: rty): Prop :=
+| closed_rty_: lc_rty ρ -> rty_fv ρ ⊆ d -> closed_rty d ρ.
+
+Lemma closed_rty_fine: forall d τ, closed_rty d τ -> fine_rty τ.
+Proof.
+  pose lc_rty_fine.
+  induction 1; eauto.
+Qed.
+
+(** Well-formedness of type context. All terms and types are alpha-converted to
+  have unique names.
+  all rty in ctx are pure.
+ *)
+Inductive ok_ctx: listctx rty -> Prop :=
+| ok_ctx_nil: ok_ctx []
+| ok_ctx_cons: forall (Γ: listctx rty)(x: atom) (ρ: rty),
+    ok_ctx Γ ->
+    closed_rty (ctxdom Γ) ρ ->
+    x ∉ ctxdom Γ ->
+    ok_ctx (Γ ++ [(x, ρ)]).
+
+(** Shorthands, used in typing rules *)
+Definition mk_eq_constant c := [: ty_of_const c | b0:c= c ].
+Definition mk_eq_constant_over c := {: ty_of_const c | b0:c= c }.
+Definition mk_bot ty := [: ty | mk_q_under_bot ].
+Definition mk_top ty := [: ty | mk_q_under_top ].
+Definition mk_eq_var ty (x: atom) := [: ty | b0:x= x ].
