WellFormedness/WfRty.v
@@ -1,0 +1,205 @@
+Require Import Stdlib.Program.Wf.
+From stdpp Require Import mapset.
+From stdpp Require Import natmap.
+From CT Require Import Syntax.RefinementType.
+
+Import BaseDef.
+Import Lang.
+Import Tactics.
+Import Primitives.
+(* Import OperationalSemantics. *)
+(* Import BasicTyping. *)
+Import Qualifier.
+Import ListCtx.
+Import List.
+
+Lemma ok_ctx_ok: forall Γ, ok_ctx Γ -> ok Γ.
+Proof.
+  induction 1; eauto.
+Qed.
+
+Lemma is_over_base_open_rty: forall τ k (v_x: value), is_over_base_rty ({ k ~> v_x} τ) <-> is_over_base_rty τ.
+Proof.
+  split; induction τ; simpl; intros; inversion H; subst; eauto.
+Qed.
+
+Lemma is_over_base_rty_subst: forall τ x (v_x: value), is_over_base_rty ({ x := v_x} τ) <-> is_over_base_rty τ.
+Proof.
+  split; induction τ; simpl; intros; inversion H; subst; eauto.
+Qed.
+
+Lemma is_under_base_open_rty: forall τ k (v_x: value), is_under_base_rty ({ k ~> v_x} τ) <-> is_under_base_rty τ.
+Proof.
+  split; induction τ; simpl; intros; inversion H; subst; eauto.
+Qed.
+
+Lemma is_under_base_rty_subst: forall τ x (v_x: value), is_under_base_rty ({ x := v_x} τ) <-> is_under_base_rty τ.
+Proof.
+  split; induction τ; simpl; intros; inversion H; subst; eauto.
+Qed.
+
+Lemma rty_measure_gt_0 ρ : rty_measure ρ > 0.
+Proof.
+  induction ρ; simpl; lia.
+Qed.
+
+Lemma rty_measure_S ρ : exists n, rty_measure ρ = S n.
+Proof.
+  destruct (Nat.lt_exists_pred 0 (rty_measure ρ)).
+  pose proof (rty_measure_gt_0 ρ). lia.
+  intuition eauto.
+Qed.
+
+Lemma open_preserves_rty_measure ρ: forall k t,
+    rty_measure ρ = rty_measure ({k ~> t} ρ).
+Proof.
+  induction ρ; simpl; eauto.
+Qed.
+
+Lemma subst_preserves_rty_measure ρ: forall x t,
+    rty_measure ρ = rty_measure ({x:=t} ρ).
+Proof.
+  induction ρ; simpl; eauto.
+Qed.
+
+Lemma is_coverage_open_rty_aux n: forall τ, rty_measure τ <= n -> forall k (v_x: value), is_coverage_rty ({ k ~> v_x} τ) <-> is_coverage_rty τ.
+Proof.
+  induction n; split; intros HH.
+  - destruct τ; sinvert H.
+  - destruct τ; sinvert H.
+  - destruct τ.
+    + sinvert HH; eauto.
+    + sinvert HH; eauto.
+    + destruct τ1; sinvert HH; eauto; econstructor; rewrite <- IHn; eauto; simpl in *; lia.
+  - destruct τ.
+    + sinvert HH; eauto.
+    + simpl. eauto.
+    + destruct τ1; sinvert HH; eauto; simpl; econstructor; try solve [rewrite IHn; eauto; simpl in *; lia].
+      * rewrite <- IHn in H2; eauto; simpl in *; lia.
+Qed.
+
+Lemma is_coverage_open_rty: forall τ, forall k (v_x: value), is_coverage_rty ({ k ~> v_x} τ) <-> is_coverage_rty τ.
+Proof. eauto using is_coverage_open_rty_aux. Qed.
+
+Lemma is_coverage_rty_subst_aux n: forall τ, rty_measure τ <= n -> forall x (v_x: value), is_coverage_rty ({ x := v_x} τ) <-> is_coverage_rty τ.
+Proof.
+  induction n; split; intros HH.
+  - destruct τ; sinvert H.
+  - destruct τ; sinvert H.
+  - destruct τ.
+    + sinvert HH; eauto.
+    + sinvert HH; eauto.
+    + destruct τ1; sinvert HH; eauto; econstructor; rewrite <- IHn; eauto; simpl in *; lia.
+  - destruct τ.
+    + sinvert HH; eauto.
+    + simpl. eauto.
+    + destruct τ1; sinvert HH; eauto; simpl; econstructor; try solve [rewrite IHn; eauto; simpl in *; lia].
+      * rewrite <- IHn in H2; eauto; simpl in *; lia.
+Qed.
+
+Lemma is_coverage_rty_subst: forall τ x (v_x: value), is_coverage_rty ({ x := v_x} τ) <-> is_coverage_rty τ.
+Proof. eauto using is_coverage_rty_subst_aux. Qed.
+
+Lemma open_rty_arr_rev: forall ρ τ k v, (({k ~> v} ρ) ⇨ ({S k ~> v} τ)) = {k ~> v} (ρ ⇨ τ).
+Proof. eauto. Qed.
+
+Lemma rty_subst_arr_rev: forall ρ τ x v, (({x := v} ρ) ⇨ ({x := v} τ)) = {x := v} (ρ ⇨ τ).
+Proof. eauto. Qed.
+
+Ltac fine_rty_aux_simp_aux :=
+  match goal with
+  | [H: context [ (({?k ~> ?v} _) ⇨ ({S ?k ~> ?v} _)) ] |- _ ] =>
+      setoid_rewrite open_rty_arr_rev in H
+  | [H: context [ (({?x := ?v} _) ⇨ ({?x := ?v} _)) ] |- _ ] =>
+      setoid_rewrite rty_subst_arr_rev in H
+  | [H: _ |- context [ (({?k ~> ?v} _) ⇨ ({S ?k ~> ?v} _)) ]] =>
+      setoid_rewrite open_rty_arr_rev
+  | [H: _ |- context [ (({?x := ?v} _) ⇨ ({?x := ?v} _)) ] ] =>
+      setoid_rewrite rty_subst_arr_rev
+  | [H: context [ is_over_base_rty ({_ ~> _} ?τ) ] |- _ ] => setoid_rewrite is_over_base_open_rty in H
+  | [H: context [ is_over_base_rty ({_ := _} ?τ) ] |- _ ] => setoid_rewrite is_over_base_rty_subst in H
+  | [H: _ |- context [ is_over_base_rty ({_ ~> _} ?τ) ] ] => setoid_rewrite is_over_base_open_rty
+  | [H: _ |- context [ is_over_base_rty ({_ := _} ?τ) ] ] => setoid_rewrite is_over_base_rty_subst
+  | [H: context [ is_under_base_rty ({_ ~> _} ?τ) ] |- _ ] => setoid_rewrite is_under_base_open_rty in H
+  | [H: context [ is_under_base_rty ({_ := _} ?τ) ] |- _ ] => setoid_rewrite is_under_base_rty_subst in H
+  | [H: _ |- context [ is_under_base_rty ({_ ~> _} ?τ) ] ] => setoid_rewrite is_under_base_open_rty
+  | [H: _ |- context [ is_under_base_rty ({_ := _} ?τ) ] ] => setoid_rewrite is_under_base_rty_subst
+  | [H: context [ is_coverage_rty ({_ ~> _} ?τ) ] |- _ ] => setoid_rewrite is_coverage_open_rty in H
+  | [H: context [ is_coverage_rty ({_ := _} ?τ) ] |- _ ] => setoid_rewrite is_coverage_rty_subst in H
+  | [H: _ |- context [ is_coverage_rty ({_ ~> _} ?τ) ] ] => setoid_rewrite is_coverage_open_rty
+  | [H: _ |- context [ is_coverage_rty ({_ := _} ?τ) ] ] => setoid_rewrite is_coverage_rty_subst
+  end.
+
+Lemma fine_open_rty τ: forall k (v_x: value), fine_rty ({ k ~> v_x} τ) <-> fine_rty τ.
+Proof.
+  split; intros; destruct τ; simpl in *; repeat fine_rty_aux_simp_aux; eauto.
+Qed.
+
+Lemma fine_rty_subst: forall τ x (v_x: value), fine_rty ({ x := v_x} τ) <-> fine_rty τ.
+Proof.
+  split; intros; destruct τ; simpl in *; repeat fine_rty_aux_simp_aux; eauto.
+Qed.
+
+Ltac fine_rty_simp_aux :=
+  match goal with
+  | [H: context [ (({?k ~> ?v} _) ⇨ ({S ?k ~> ?v} _)) ] |- _ ] =>
+      setoid_rewrite open_rty_arr_rev in H
+  | [H: context [ (({?x := ?v} _) ⇨ ({?x := ?v} _)) ] |- _ ] =>
+      setoid_rewrite rty_subst_arr_rev in H
+  | [H: _ |- context [ (({?k ~> ?v} _) ⇨ ({S ?k ~> ?v} _)) ]] =>
+      setoid_rewrite open_rty_arr_rev
+  | [H: _ |- context [ (({?x := ?v} _) ⇨ ({?x := ?v} _)) ] ] =>
+      setoid_rewrite rty_subst_arr_rev
+  | [H: context [ fine_rty ({_ ~> _} ?τ) ] |- _ ] => setoid_rewrite fine_open_rty in H
+  | [H: context [ fine_rty ({_ := _} ?τ) ] |- _ ] => setoid_rewrite fine_rty_subst in H
+  | [H: _ |- context [ fine_rty ({_ ~> _} ?τ) ] ] => setoid_rewrite fine_open_rty
+  | [H: _ |- context [ fine_rty ({_ := _} ?τ) ] ] => setoid_rewrite fine_rty_subst
+  | _ => fine_rty_aux_simp_aux
+  end.
+
+Lemma lc_rty_under_base_q: forall b ϕ, lc_rty ([:b|ϕ]) <-> lc_phi1 ϕ.
+Proof.
+  split; intros; sinvert H; eauto.
+  econstructor; eauto. exists x. eauto. simpl; eauto.
+Qed.
+
+Lemma lc_rty_over_base_q: forall b ϕ, lc_rty ({:b|ϕ}) <-> lc_phi1 ϕ.
+Proof.
+  split; intros; sinvert H; eauto.
+  econstructor; eauto. exists x. eauto. simpl; eauto.
+Qed.
+
+Lemma lc_rty_base_flip: forall b ϕ, lc_rty {:b|ϕ} <-> lc_rty [:b|ϕ].
+Proof.
+  split; intros; sinvert H; econstructor; eauto.
+Qed.
+
+Lemma closed_rty_base_flip: forall L b ϕ, closed_rty L {:b|ϕ} <-> closed_rty L [:b|ϕ].
+Proof.
+  split; intros; sinvert H; econstructor; eauto;
+  rewrite lc_rty_base_flip in *; eauto.
+Qed.
+
+Lemma lc_rty_arr: forall ρ τ, lc_rty (ρ ⇨ τ) <-> fine_rty (ρ ⇨ τ) /\ lc_rty ρ /\ body_rty τ.
+Proof.
+  split; intros; sinvert H.
+  - intuition. auto_exists_L.
+  - unfold body_rty in H1. simp_hyps. auto_exists_L; eauto.
+Qed.
+
+Lemma closed_rty_arr:
+  ∀ (L : aset) (ρ τ : rty),
+    closed_rty L (ρ⇨τ) ↔ (fine_rty (ρ⇨τ)) /\ closed_rty L ρ ∧ body_rty τ /\ (rty_fv τ ⊆ L).
+Proof.
+  split; intros.
+  - sinvert H. rewrite lc_rty_arr in H0. intuition.
+    + econstructor; eauto. my_set_solver.
+    + my_set_solver.
+  - simp_hyps. sinvert H1. econstructor; eauto.
+    + rewrite lc_rty_arr. intuition.
+    + my_set_solver.
+Qed.
+
+Ltac fine_rty_simp := simpl in *; repeat fine_rty_simp_aux.
+
+Ltac fine_rty_solver := fine_rty_simp; eauto.
